Fix erasure proof

erasure.v
@@ -6,46 +6,52 @@ From stdpp Require Import gmap.
 
 Definition have_same_proph
            (σ : language.state P_lang) (σ' : language.state PE_lang)
-  := σ.1 = σ'.1 ∧ dom (gset loc) σ.2 = σ'.2.
+  := (Heap σ) = (EHeap σ') ∧ dom (gset loc) (Proph σ) = (EProph σ') ∧
+     (ioState σ) = (EioState σ').
 
 Definition conjure_prophecies (σ : language.state PE_lang) :
   language.state P_lang :=
-  match σ with
-    (σh, σp) => (σh,  to_gmap (Sconst UnitV) σp)
-  end.
+  {| Heap := EHeap σ; Proph := to_gmap (Sconst UnitV) (EProph σ);
+     ioState := EioState σ |}.
 
 Lemma conjure_prophecies_have_same_proph σ :
   have_same_proph (conjure_prophecies σ) σ.
 Proof.
-  destruct σ; split; first done; simpl.
+  destruct σ as [h p i]; split; first done; simpl.
+  split; last done.
   apply mapset.mapset_eq => x; split => Hx.
-  - destruct (decide (x ∈ m)); first done.
+  - destruct (decide (x ∈ p)); first done.
     apply elem_of_dom in Hx. destruct Hx as [y Hy].
     rewrite lookup_to_gmap option_guard_False //= in Hy.
   - apply elem_of_dom. rewrite lookup_to_gmap option_guard_True; eauto.
 Qed.
 
 Lemma erased_reachable_reachable th1 h1 th2 σ2:
-  rtc (@step PE_lang) (th1, (h1, ∅)) (th2, σ2) →
+  rtc (@step PE_lang) (th1, {| EHeap := h1; EProph := ∅; EioState := (λ _, False) |})
+(th2, σ2) →
   ∀ σ2', have_same_proph σ2' σ2 →
-         rtc (@step P_lang) (th1, (h1, ∅)) (th2, σ2').
+         rtc (@step P_lang)
+             (th1, {| Heap := h1; Proph := ∅; ioState := (λ _, False) |})
+             (th2, σ2').
 Proof.
-  remember (th1, (h1, ∅)) as cfg.
+  remember (th1, {| EHeap := h1; EProph := ∅; EioState := (λ _, False) |}) as cfg.
   remember (th2, σ2) as cfg'.
   intros Hrtc.
   revert th1 h1 th2 σ2 Heqcfg Heqcfg'.
   eapply (rtc_ind_r_weak (λ z z', ∀ (th1 : list (language.expr PE_lang)) (h1 : gmap loc val)
                                     (th2 : list (language.expr PE_lang))
                                     (σ2 : language.state PE_lang),
-                             z = (th1, (h1, ∅))
+                             z = (th1, {| EHeap := h1; EProph := ∅; EioState := (λ _, False) |})
                              → z' = (th2, σ2) →
                              ∀ σ2' : language.state P_lang,
                                have_same_proph σ2' σ2 →
-                               rtc (@step P_lang) (th1, (h1, ∅)) (th2, σ2')));
+                               rtc (@step P_lang)
+                                   (th1, {| Heap := h1; Proph := ∅;
+                                            ioState := (λ _, False) |}) (th2, σ2')));
   last eauto.
   - intros x th1 h1 th2 σ2 Heqcfg Heqcfg'; simplify_eq.
-    intros [σ2 σ2p] [Hh Hsp]; simpl in *.
-    rewrite Hh. rewrite (dom_empty_inv_L (D := gset loc) σ2p); last done.
+    intros [σ2 σ2p σ2i] [Hh [Hsp Hi]]; simpl in *; simplify_eq.
+    rewrite (dom_empty_inv_L (D := gset loc) σ2p); last done.
     econstructor.
   - intros x y z Hxy Hyz IH th1 h1 th2 σ2 Heqcfg Heqcfg' σ2' Hsp;
       simplify_eq; simpl in *.
@@ -53,60 +59,61 @@ Proof.
     inversion Hyz as [? ? ? ? ? ? ? ? ? Hpr]; simplify_eq.
     inversion Hpr as [? ? ? ? ? Hestp]; simpl in *; simplify_eq.
     inversion Hestp; simplify_eq;
-      try (eapply rtc_r; first (by eapply IH; eauto); by repeat (econstructor; eauto)).
-    all: destruct σ2' as [σ2'h σ2'p]; destruct Hsp as [Hsp1 Hsp2]; simpl in *; simplify_eq.
-    + eapply (rtc_r _ (_ ++ fill K (Alloc _) :: _, (σ, σ2'p)));
-        [unshelve eapply (IH _ _ _ (_, _) _ _ (σ, σ2'p)); eauto; split; simpl; eauto|
-         repeat (econstructor; eauto)].
-    + match goal with A : ?X.1 !! _ = _ |- _ => destruct X as [σmh σmp]; simpl in * end.
-      eapply (rtc_r _ (_ ++ fill K (Load (Loc _)) :: _, (_, σ2'p)));
-        [unshelve eapply (IH _ _ _ (σmh, σmp) _ _ (_, σ2'p)); eauto; split; simpl; eauto|
-         repeat (econstructor; eauto)].
-    + eapply (rtc_r _ (_ ++ fill K (Store (Loc _) _) :: _, (_, σ2'p)));
-        [unshelve eapply (IH _ _ _ (_, _) _ _ (_, σ2'p)); eauto; split; simpl; eauto|
-         repeat (econstructor; eauto)].
-    + match goal with A : ?X.1 !! _ = _ |- _ => destruct X as [σmh σmp]; simpl in * end.
-      eapply (rtc_r _ (_ ++ fill K (CAS (Loc _) _ _) :: _, (_, σ2'p)));
-        [unshelve eapply (IH _ _ _ (_, _) _ _ (_, σ2'p)); eauto; split; simpl; eauto|
-         repeat (econstructor; eauto)].
-    + eapply (rtc_r _ (_ ++ fill K (CAS (Loc _) _ _) :: _, (_, σ2'p)));
-        [unshelve eapply (IH _ _ _ (_, _) _ _ (_, σ2'p)); eauto; split; simpl; eauto|
-         repeat (econstructor; eauto)].
-    + assert (({[fresh σp]} ∪ σp) ∖ {[fresh σp]} = σp) as Hfr.
+      try (eapply rtc_r; first (by eapply IH; eauto);
+             by repeat (econstructor; eauto)).
+    all: destruct σ2' as [σ2'h σ2'p σ2'i]; destruct Hsp as [Hsp1 [Hsp2 Hi]];
+      simpl in *; simplify_eq;
+    repeat match goal with
+      | H : is_Some _ |- _ => destruct H
+           end;
+    try (by (eapply (rtc_r _ (_ ++ fill K _ :: _, {| Proph := σ2'p; |}));
+             [eapply IH; by eauto |repeat econstructor; eauto])).
+    + assert (({[fresh (EProph σ1)]} ∪ (EProph σ1)) ∖ {[fresh (EProph σ1)]} =
+              (EProph σ1)) as Hfr.
       { rewrite difference_union_distr_l_L difference_diag_L left_id_L.
         apply difference_disjoint_L.
         symmetry. apply disjoint_singleton_l, is_fresh. }
-      eapply (rtc_r _ (_ ++ fill K (Create_Pr) :: _, (_, delete (fresh σp) σ2'p)));
-        [unshelve eapply (IH _ _ _ (_, _) _ _ (_, _)); eauto; split; simpl; eauto|
-         repeat (econstructor; eauto)].
-      * by rewrite (dom_delete_L (D := gset loc)) Hsp2 Hfr.
-      * destruct (elem_of_dom (D := gset loc) σ2'p (fresh σp)) as [[str Hstr]].
+      eapply (rtc_r _ (_ ++ fill K (Create_Pr) :: _,
+                       {|Proph := delete (fresh (EProph σ1)) σ2'p |})).
+      * eapply IH; eauto.
+        repeat split; eauto.
+          by rewrite (dom_delete_L (D := gset loc)) Hsp2 Hfr.
+      * destruct (elem_of_dom (D := gset loc) σ2'p (fresh (EProph σ1)))
+          as [[str Hstr]].
         { rewrite Hsp2. by apply elem_of_union_l, elem_of_singleton. }
-        replace σ2'p with (<[fresh (dom (gset loc) (delete (fresh σp) σ2'p)) := str]> (delete (fresh σp) σ2'p)) at 2; last first.
+        replace σ2'p with
+            (<[fresh (dom (gset loc) (delete (fresh (EProph σ1)) σ2'p))
+               := str]> (delete (fresh (EProph σ1)) σ2'p)) at 2; last first.
         { rewrite dom_delete_L Hsp2 Hfr insert_delete. by apply insert_id. }
         rewrite -{2}Hfr -Hsp2 -dom_delete_L.
-        econstructor.
+        repeat econstructor; eauto.
     + assert (∃ str, σ2'p !! l = Some str) as [str Hstr]
-          by by apply (elem_of_dom (D := gset loc)).
+          by by apply (elem_of_dom (D := gset loc)); rewrite Hsp2.
       eapply (rtc_r _ (_ ++ fill K (Assign_Pr (Pr _) _) :: _,
-                       (_, <[l:={| Shead := v; Stail := str|}]> σ2'p)));
-        [unshelve eapply (IH _ _ _ (_, _) _ _ (_, _)); eauto; split; simpl; eauto|
-         repeat (econstructor; eauto)].
-      * rewrite dom_insert_L. by apply subseteq_union_1_L, elem_of_subseteq_singleton.
-      * replace σ2'p with (<[l:= Stail {| Shead := v; Stail := str |}]>(<[l:={| Shead := v; Stail := str |}]> σ2'p)) at 2; last first.
+                       {| Proph := <[l:={| Shead := v; Stail := str|}]> σ2'p|})).
+      * eapply IH; eauto.
+        repeat split; simpl; eauto.
+        rewrite dom_insert_L.
+        rewrite Hsp2 subseteq_union_1_L; first by auto.
+        by apply elem_of_subseteq_singleton.
+      * replace σ2'p with
+            (<[l:= Stail {| Shead := v; Stail := str |}]>
+             (<[l:={| Shead := v; Stail := str |}]> σ2'p)) at 2; last first.
         { rewrite /= insert_insert. by apply insert_id. }
-        econstructor; auto.
+        repeat econstructor; auto.
         rewrite lookup_insert //.
 Qed.
 
 Definition safe e :=
   ∀ th2 σ2,
-    rtc (@step P_lang) ([e], (∅, ∅)) (th2, σ2) →
+    rtc (@step P_lang) ([e], {| Heap := ∅; Proph := ∅; ioState := (λ _, False) |})
+        (th2, σ2) →
     ∀ e, e ∈ th2 → AsVal e ∨ reducible e σ2.
 
 Definition erased_safe e :=
   ∀ th2 σ2,
-    rtc (@step PE_lang) ([e], (∅, ∅)) (th2, σ2) →
+    rtc (@step PE_lang) ([e], {| EHeap := ∅; EProph := ∅; EioState := (λ _, False) |})
+        (th2, σ2) →
     ∀ e, e ∈ th2 → AsVal e ∨ reducible e σ2.
 
 Lemma reducible_erase_reducible e σ σ' :
@@ -117,22 +124,24 @@ Proof.
   intros Hsp (e'&σ2&efs&Hrd); simpl in *.
   inversion Hrd as [K e1' e2' ? ? Hhrd]; simpl in *; subst.
   destruct σ as [σh σp]; destruct σ' as [σ'h σ'p];
-    destruct Hsp as [? ?]; simpl in *; simplify_eq.
-  inversion Hhrd; subst; try (unshelve (repeat econstructor; eauto); fail).
-  + match goal with A : is_Some _ |- _ => destruct A as [? ?] end.
-    repeat econstructor; eauto.
-  + repeat econstructor; eauto.
+    destruct Hsp as [? [? ?]]; simpl in *; simplify_eq.
+  inversion Hhrd; subst; try (unshelve (repeat econstructor; eauto); fail);
+    repeat match goal with A : is_Some _ |- _ => destruct A as [? ?] end;
+    simpl in *.
+  - repeat econstructor; eauto.
+  - repeat econstructor; simpl; eauto.
     apply elem_of_dom; eauto.
-  + repeat econstructor; eauto.
+  - repeat econstructor; eauto.
     apply elem_of_dom; eauto.
-  + by unshelve (repeat econstructor).
+  - by unshelve (repeat econstructor).
 Qed.
 
 Lemma soundness_prophecies e :
   safe e → erased_safe e.
 Proof.
   intros Hs th2 σ2 Hrtc re Hre.
-  assert (rtc step ([e], (∅, ∅)) (th2, conjure_prophecies σ2)) as Hrtc'.
+  assert (rtc step ([e], {| Heap := ∅; Proph := ∅; ioState := (λ _, False) |})
+              (th2, conjure_prophecies σ2)) as Hrtc'.
   { eapply erased_reachable_reachable;
       eauto using conjure_prophecies_have_same_proph. }
   edestruct Hs as [?|Hred]; eauto.
