lang_erased.v
@@ -6,7 +6,20 @@ From stdpp Require Import gmap.
 
 Module Plang_erased.
 
-  Definition erased_state : Type := (gmap loc val) * (gset loc).
+  Record erased_state : Type :=
+    { EHeap : gmap loc val;
+      EProph : (gset loc);
+      EioState : ioSpec
+    }.
+
+  Definition update_Eheap σ h :=
+    {| EHeap := h; EProph := EProph σ; EioState := EioState σ |}.
+
+  Definition update_Eproph σ ι :=
+    {| EHeap := EHeap σ; EProph := ι; EioState := EioState σ |}.
+
+  Definition update_EioState σ T :=
+    {| EHeap := EHeap σ; EProph := EProph σ; EioState := T |}.
 
   Inductive erased_head_step :
     expr → erased_state → expr → erased_state → list expr → Prop :=
@@ -14,6 +27,15 @@ Module Plang_erased.
   | EBetaS e1 e2 v2 σ :
       to_val e2 = Some v2 →
       erased_head_step (App (Rec e1) e2) σ e1.[(Rec e1), e2/] σ []
+  | EZetaS e1 e2 v1 σ :
+      to_val e1 = Some v1 →
+      erased_head_step (LetIn e1 e2) σ e2.[e1/] σ []
+  | ELamBetaS e1 e2 v2 σ :
+      to_val e2 = Some v2 →
+      erased_head_step (App (Lam e1) e2) σ e1.[e2/] σ []
+  | ESeqS e1 e2 v1 σ :
+      to_val e1 = Some v1 →
+      erased_head_step (Seq e1 e2) σ e2 σ []
   (* Products *)
   | EFstS e1 v1 e2 v2 σ :
       to_val e1 = Some v1 → to_val e2 = Some v2 →
@@ -47,32 +69,35 @@ Module Plang_erased.
   | EForkS e σ:
       erased_head_step (Fork e) σ Unit σ [e]
   (* Reference Types *)
-  | EAllocS e v σ σp l :
-     to_val e = Some v → σ !! l = None →
-     erased_head_step (Alloc e) (σ, σp) (Loc l) (<[l:=v]>σ, σp) []
+  | EAllocS e v σ l :
+     to_val e = Some v → (EHeap σ) !! l = None →
+     erased_head_step (Alloc e) σ (Loc l) (update_Eheap σ (<[l:=v]>(EHeap σ))) []
   | ELoadS l v σ :
-     σ.1 !! l = Some v →
+     (EHeap σ) !! l = Some v →
      erased_head_step (Load (Loc l)) σ (of_val v) σ []
-  | EStoreS l e v σ σp :
-     to_val e = Some v → is_Some (σ !! l) →
-     erased_head_step (Store (Loc l) e) (σ, σp) Unit (<[l:=v]>σ, σp) []
+  | EStoreS l e v σ :
+     to_val e = Some v → is_Some ((EHeap σ) !! l) →
+     erased_head_step (Store (Loc l) e) σ Unit (update_Eheap σ (<[l:=v]>(EHeap σ))) []
   (* Compare and swap *)
   | ECasFailS l e1 v1 e2 v2 vl σ :
      to_val e1 = Some v1 → to_val e2 = Some v2 →
-     σ.1 !! l = Some vl → vl ≠ v1 →
+     (EHeap σ) !! l = Some vl → vl ≠ v1 →
      erased_head_step (CAS (Loc l) e1 e2) σ (#♭ false) σ []
-  | ECasSucS l e1 v1 e2 v2 σ σp :
+  | ECasSucS l e1 v1 e2 v2 σ :
      to_val e1 = Some v1 → to_val e2 = Some v2 →
-     σ !! l = Some v1 →
-     erased_head_step (CAS (Loc l) e1 e2) (σ, σp) (#♭ true) (<[l:=v2]>σ, σp) []
+     (EHeap σ) !! l = Some v1 →
+     erased_head_step (CAS (Loc l) e1 e2) σ (#♭ true) (update_Eheap σ (<[l:=v2]>(EHeap σ))) []
   (* Prophecy operational semantics *)
-  | ECreate_PrS σ σp :
-      erased_head_step Create_Pr (σ, σp) (Pr (fresh σp))
-                (σ, {[fresh σp]} ∪ σp) []
-  | EAssignS v l e σ σp :
-     l ∈ σp → to_val e = Some v →
-     erased_head_step (Assign_Pr (Pr l) e) (σ, σp) Unit (σ, σp) []
-  | ERandS b σ : erased_head_step Rand σ (Bool b) σ [].
+  | ECreate_PrS σ :
+      erased_head_step Create_Pr σ (Pr (fresh (EProph σ)))
+                       (update_Eproph σ ({[fresh (EProph σ)]} ∪ (EProph σ))) []
+  | EAssignS v l e σ :
+     l ∈ (EProph σ) → to_val e = Some v →
+     erased_head_step (Assign_Pr (Pr l) e) σ Unit σ []
+  | ERandS b σ : erased_head_step Rand σ (Bool b) σ []
+  | EIOS t e v v' σ : to_val e = Some v → (EioState σ) [(t, v, v')] →
+                    erased_head_step (IO t e) σ (of_val v')
+                              (update_EioState σ (λ τ, (EioState σ) ((t, v, v') :: τ))) [].
 
   (** Basic properties about the language *)
   Lemma val_stuck e1 σ1 e2 σ2 ef :
@@ -83,9 +108,10 @@ Module Plang_erased.
     erased_head_step (fill_item Ki e) σ1 e2 σ2 ef → is_Some (to_val e).
   Proof. destruct Ki; inversion_clear 1; simplify_option_eq; eauto. Qed.
 
-  Lemma alloc_fresh e v σ σp :
-    let l := fresh (dom (gset loc) σ) in
-    to_val e = Some v → erased_head_step (Alloc e) (σ, σp) (Loc l) (<[l:=v]>σ, σp) [].
+  Lemma alloc_fresh e v σ :
+    let l := fresh (dom (gset loc) (EHeap σ)) in
+    to_val e = Some v → erased_head_step (Alloc e) σ (Loc l)
+                                         (update_Eheap σ (<[l:=v]>(EHeap σ))) [].
   Proof. by intros; apply EAllocS, (not_elem_of_dom (D:=gset loc)), is_fresh. Qed.
 
   Lemma val_head_stuck e1 σ1 e2 σ2 efs : erased_head_step e1 σ1 e2 σ2 efs → to_val e1 = None.
