lang.v
@@ -21,6 +21,7 @@ Module Plang.
   | Rec (e : {bind 2 of expr})
   | Lam (e : {bind expr})
   | LetIn (e : expr) (e : {bind expr})
+  | Seq (e1 e2 : expr)
   | App (e1 e2 : expr)
   (* Base Types *)
   | Unit
@@ -143,6 +144,7 @@ Module Plang.
   | AppLCtx (e2 : expr)
   | AppRCtx (v1 : val)
   | LetInCtx (e2 : expr)
+  | SeqCtx (e2 : expr)
   | TAppCtx
   | PairLCtx (e2 : expr)
   | PairRCtx (v1 : val)
@@ -172,6 +174,7 @@ Module Plang.
     | AppLCtx e2 => App e e2
     | AppRCtx v1 => App (of_val v1) e
     | LetInCtx e2 => LetIn e e2
+    | SeqCtx e2 => Seq e e2
     | TAppCtx => TApp e
     | PairLCtx e2 => Pair e e2
     | PairRCtx v1 => Pair (of_val v1) e
@@ -235,6 +238,9 @@ Module Plang.
   | LamBetaS e1 e2 v2 σ :
       to_val e2 = Some v2 →
       head_step (App (Lam e1) e2) σ e1.[e2/] σ []
+  | SeqS e1 e2 v1 σ :
+      to_val e1 = Some v1 →
+      head_step (Seq e1 e2) σ e2 σ []
   (* Products *)
   | FstS e1 v1 e2 v2 σ :
       to_val e1 = Some v1 → to_val e2 = Some v2 →
