rules.v
@@ -343,6 +343,10 @@ Section lang_rules.
     PureExec True (LetIn e1 e2) e2.[e1 /].
   Proof. solve_pure_exec. Qed.
 
+  Global Instance pure_Seq e1 e2 `{!AsVal e1} :
+    PureExec True (Seq e1 e2) e2.
+  Proof. solve_pure_exec. Qed.
+
   Global Instance pure_tlam e : PureExec True (TApp (TLam e)) e.
   Proof. solve_pure_exec. Qed.
 
